functorization for tree aggregation

systems/TreeAggregationStatic.v
@@ -27,30 +27,32 @@ Require Import Sorting.Permutation.
 
 Require Import AAC_tactics.AAC.
 
-Require Import FailureRecorderStatic.
 Require Import AggregationStatic.
 
 Set Implicit Arguments.
 
-Class NameOverlayRootParams `(N : NameOverlayParams) :=
-  {
-    root : name -> Prop ;
-    root_dec : forall n, {root n} + {~ root n} ;
-    root_unique : forall n n', root n -> root n' -> n = n'
-  }.
+Module Type RootNameType (Import NT : NameType).
+Parameter root : name -> Prop.
+Parameter root_dec : forall n, {root n} + {~ root n}.
+Parameter root_unique : forall n n', root n -> root n' -> n = n'.
+End RootNameType.
 
-Module TreeAggregation (N : NatValue) (CFG : CommutativeFinGroup).
+Module TreeAggregation (Import NT : NameType) 
+ (Import ANT : AdjacentNameType NT) (Import RNT : RootNameType NT)
+ (NOT : NameOrderedType NT) (NSet : MSetInterface.S with Module E := NOT) 
+ (NOTC : NameOrderedTypeCompat NT) (NMap : FMapInterface.S with Module E := NOTC) 
+ (Import CFG : CommutativeFinGroup).
 
-Module AGN := Aggregation N CFG.
-Import AGN.FRN.AN.
+Module AN := Adjacency NT ANT NOT NSet.
+Import AN.
 
-Import CFG.
+Module AGN := Aggregation NT ANT NOT NSet NOTC NMap CFG.
 
 Import GroupScope.
 
-Module FinNSetFacts := Facts FinNSet.
-Module FinNSetProps := Properties FinNSet.
-Module FinNSetOrdProps := OrdProperties FinNSet.
+Module NSetFacts := Facts NSet.
+Module NSetProps := Properties NSet.
+Module NSetOrdProps := OrdProperties NSet.
 
 Definition m := gT.
 
@@ -108,25 +110,20 @@ case: o; case: o0.
 - by left.
 Defined.
 
-Definition FinNM := FinNMap.t m.
-Definition FinNL := FinNMap.t nat.
+Definition NM := NMap.t m.
+Definition NL := NMap.t nat.
 
 Record Data :=  mkData { 
   local : m ; 
   aggregate : m ; 
-  adjacent : FinNS ; 
-  sent : FinNM ; 
-  received : FinNM ;
+  adjacent : NS ; 
+  sent : NM ; 
+  received : NM ;
   broadcast : bool ; 
-  levels : FinNL 
+  levels : NL
 }.
 
 Definition init_map := AGN.init_map.
-
-Section RootAdjacency.
-
-Context {fin_nop : NameOverlayParams Fin_n_NameParams}.
-Context {root_params : NameOverlayRootParams fin_nop}.
 
 Definition InitData (n : name) := 
 if root_dec n then
@@ -136,7 +133,7 @@ if root_dec n then
      sent := init_map (adjacency n nodes) ;
      received := init_map (adjacency n nodes) ;
      broadcast := true ;
-     levels := FinNMap.empty lv |}
+     levels := NMap.empty lv |}
 else
   {| local := 1 ;
      aggregate := 1 ;
@@ -144,26 +141,26 @@ else
      sent := init_map (adjacency n nodes) ;
      received := init_map (adjacency n nodes) ;
      broadcast := false ;
-     levels := FinNMap.empty lv |}.
-                            
-Inductive level_in (fs : FinNS) (fl : FinNL) (n : name) (lv' : lv) : Prop :=
-| in_level_in : FinNSet.In n fs -> FinNMap.find n fl = Some lv' -> level_in fs fl n lv'.
+     levels := NMap.empty lv |}.
 
-Inductive min_level (fs : FinNS) (fl : FinNL) (n : name) (lv' : lv) : Prop :=
+Inductive level_in (fs : NS) (fl : NL) (n : name) (lv' : lv) : Prop :=
+| in_level_in : NSet.In n fs -> NMap.find n fl = Some lv' -> level_in fs fl n lv'.
+
+Inductive min_level (fs : NS) (fl : NL) (n : name) (lv' : lv) : Prop :=
 | min_lv_min : level_in fs fl n lv' -> 
   (forall (lv'' : lv) (n' : name), level_in fs fl n' lv'' -> ~ lv'' < lv') ->
   min_level fs fl n lv'.
 
-Record st_par := mk_st_par { st_par_set : FinNS ; st_par_map : FinNL }.
+Record st_par := mk_st_par { st_par_set : NS ; st_par_map : NL }.
 
 Record nlv := mk_nlv { nlv_n : name ; nlv_lv : lv }.
 
 Definition st_par_lt (s s' : st_par) : Prop :=
-FinNSet.cardinal s.(st_par_set) < FinNSet.cardinal s'.(st_par_set).
+NSet.cardinal s.(st_par_set) < NSet.cardinal s'.(st_par_set).
 
 Lemma st_par_lt_well_founded : well_founded st_par_lt.
 Proof.
-apply (well_founded_lt_compat _ (fun s => FinNSet.cardinal s.(st_par_set))).
+apply (well_founded_lt_compat _ (fun s => NSet.cardinal s.(st_par_set))).
 by move => x y; rewrite /st_par_lt => H.
 Qed.
 
@@ -177,11 +174,11 @@ Definition par_F : forall s : st_par,
 rewrite /par_t.
 refine 
   (fun (s : st_par) par_rec => 
-   match FinNSet.choose s.(st_par_set) as sopt return (_ = sopt -> _) with
+   match NSet.choose s.(st_par_set) as sopt return (_ = sopt -> _) with
    | Some n => fun (H_eq : _) => 
-     match par_rec (mk_st_par (FinNSet.remove n s.(st_par_set)) s.(st_par_map)) _ with
+     match par_rec (mk_st_par (NSet.remove n s.(st_par_set)) s.(st_par_map)) _ with
      | inleft (exist nlv' H_min) =>
-       match FinNMap.find n s.(st_par_map) as n' return (_ = n' -> _) with
+       match NMap.find n s.(st_par_map) as n' return (_ = n' -> _) with
        | Some lv' => fun (H_find : _) => 
          match lt_dec lv' nlv'.(nlv_lv)  with
          | left H_dec => inleft _ (exist _ (mk_nlv n lv') _)
@@ -190,7 +187,7 @@ refine
        | None => fun (H_find : _) => inleft _ (exist _ nlv' _)
        end (refl_equal _)
      | inright H_min =>
-       match FinNMap.find n s.(st_par_map) as n' return (_ = n' -> _) with
+       match NMap.find n s.(st_par_map) as n' return (_ = n' -> _) with
        | Some lv' => fun (H_find : _) => inleft _ (exist _ (mk_nlv n lv') _)
        | None => fun (H_find : _) => inright _ _
        end (refl_equal _)
@@ -198,27 +195,27 @@ refine
    | None => fun (H_eq : _) => inright _ _
    end (refl_equal _)) => /=.
 - rewrite /st_par_lt /=.
-  apply FinNSet.choose_spec1 in H_eq.
-  set sr := FinNSet.remove _ _.
-  have H_notin: ~ FinNSet.In n sr by move => H_in; apply FinNSetFacts.remove_1 in H_in.
-  have H_add: FinNSetProps.Add n sr s.(st_par_set).
-    rewrite /FinNSetProps.Add.
+  apply NSet.choose_spec1 in H_eq.
+  set sr := NSet.remove _ _.
+  have H_notin: ~ NSet.In n sr by move => H_in; apply NSetFacts.remove_1 in H_in.
+  have H_add: NSetProps.Add n sr s.(st_par_set).
+    rewrite /NSetProps.Add.
     move => n'.
     split => H_in.
-      case (fin_eq_dec _ n n') => H_eq'; first by left.
-      by right; apply FinNSetFacts.remove_2.
+      case (name_eq_dec n n') => H_eq'; first by left.
+      by right; apply NSetFacts.remove_2.
     case: H_in => H_in; first by rewrite -H_in.
-    by apply FinNSetFacts.remove_3 in H_in.
-  have H_card := FinNSetProps.cardinal_2 H_notin H_add.
+    by apply NSetFacts.remove_3 in H_in.
+  have H_card := NSetProps.cardinal_2 H_notin H_add.
   rewrite H_card {H_notin H_add H_card}.
   by auto with arith.
-- apply FinNSet.choose_spec1 in H_eq.
+- apply NSet.choose_spec1 in H_eq.
   rewrite /= {s0} in H_min.
   apply min_lv_min; first exact: in_level_in.
   move => lv'' n' H_lv.
   inversion H_lv => {H_lv}.
   inversion H_min => {H_min}.
-  case (fin_eq_dec _ n n') => H_eq'.
+  case (name_eq_dec n n') => H_eq'.
     rewrite -H_eq' in H0.
     rewrite H_find in H0.
     injection H0 => H_eq_lt.
@@ -227,45 +224,45 @@ refine
   suff H_suff: ~ lv'' < nlv'.(nlv_lv) by omega.
   apply: (H2 _ n').
   apply: in_level_in => //.
-  by apply FinNSetFacts.remove_2.
-- apply FinNSet.choose_spec1 in H_eq.
+  by apply NSetFacts.remove_2.
+- apply NSet.choose_spec1 in H_eq.
   rewrite /= {s0} in H_min.
   inversion H_min => {H_min}.
   inversion H => {H}.
   apply min_lv_min.
     apply: in_level_in => //.
-    by apply FinNSetFacts.remove_3 in H1.
+    by apply NSetFacts.remove_3 in H1.
   move => lv'' n' H_lv.
   inversion H_lv => {H_lv}.
-  case (fin_eq_dec _ n n') => H_eq'.
+  case (name_eq_dec n n') => H_eq'.
     rewrite -H_eq' in H3.
     rewrite H_find in H3.
     injection H3 => H_eq_lv.
     by rewrite -H_eq_lv.
   apply: (H0 _ n').
   apply: in_level_in => //.
-  exact: FinNSetFacts.remove_2.
-- apply FinNSet.choose_spec1 in H_eq.
+  exact: NSetFacts.remove_2.
+- apply NSet.choose_spec1 in H_eq.
   rewrite /= {s0} in H_min.
   inversion H_min => {H_min}.
   inversion H => {H}.
   apply min_lv_min.
     apply: in_level_in => //.
-    by apply FinNSetFacts.remove_3 in H1.
+    by apply NSetFacts.remove_3 in H1.
   move => lv' n' H_lv.
   inversion H_lv => {H_lv}.
-  case (fin_eq_dec _ n n') => H_eq'.
+  case (name_eq_dec n n') => H_eq'.
     rewrite -H_eq' in H3.
     by rewrite H_find in H3.
   apply: (H0 _ n').
   apply: in_level_in => //.
-  exact: FinNSetFacts.remove_2.
-- apply FinNSet.choose_spec1 in H_eq.
+  exact: NSetFacts.remove_2.
+- apply NSet.choose_spec1 in H_eq.
   rewrite /= in H_min.
   apply min_lv_min; first exact: in_level_in.
   move => lv'' n' H_lv.
   inversion H_lv.
-  case (fin_eq_dec _ n n') => H_eq'.
+  case (name_eq_dec n n') => H_eq'.
     rewrite -H_eq' in H0.
     rewrite H_find in H0.
     injection H0 => H_eq_lv.
@@ -275,19 +272,19 @@ refine
   case: H_min.
   exists (mk_nlv n' lv'') => /=.
   apply: in_level_in => //.
-  exact: FinNSetFacts.remove_2.
-- apply FinNSet.choose_spec1 in H_eq.
+  exact: NSetFacts.remove_2.
+- apply NSet.choose_spec1 in H_eq.
   rewrite /= in H_min.
   move => [nlv' H_lv].
   inversion H_lv => {H_lv}.
   case: H_min.
   exists nlv'.
-  case (fin_eq_dec _ n nlv'.(nlv_n)) => H_eq'.
+  case (name_eq_dec n nlv'.(nlv_n)) => H_eq'.
     rewrite -H_eq' in H0.
     by rewrite H_find in H0.
   apply: in_level_in => //.
-  exact: FinNSetFacts.remove_2.
-- apply FinNSet.choose_spec2 in H_eq.
+  exact: NSetFacts.remove_2.
+- apply NSet.choose_spec2 in H_eq.
   move => [nlv' H_lv].
   inversion H_lv => {H_lv}.
   by case (H_eq nlv'.(nlv_n)).
@@ -318,13 +315,13 @@ refine
   by exists (mk_nlv n lv').
 Defined.
 
-Definition parent (fs : FinNS) (fl : FinNL) : option name :=
+Definition parent (fs : NS) (fl : NL) : option name :=
 match par (mk_st_par fs fl) with
 | inleft (exist nlv' _) => Some nlv'.(nlv_n)
 | inright _ => None
 end.
 
-Definition level (fs : FinNS) (fl : FinNL) : option lv :=
+Definition level (fs : NS) (fl : NL) : option lv :=
 match lev (mk_st_par fs fl) with
 | inleft (exist lv' _) => Some lv'
 | inright _ => None
@@ -341,32 +338,32 @@ Definition RootNetHandler (src : name) (msg : Msg) : Handler Data :=
 st <- get ;;
 match msg with 
 | Aggregate m_msg => 
-  match FinNMap.find src st.(received) with
+  match NMap.find src st.(received) with
   | None => nop
   | Some m_src => 
     put {| local := st.(local) ;
            aggregate := st.(aggregate) * m_msg ;
            adjacent := st.(adjacent) ;
            sent := st.(sent) ;
-           received := FinNMap.add src (m_src * m_msg) st.(received) ;
+           received := NMap.add src (m_src * m_msg) st.(received) ;
            broadcast := st.(broadcast) ;
            levels := st.(levels) |}
   end
 | Level _ => nop 
 | Fail => 
-  match FinNMap.find src st.(sent), FinNMap.find src st.(received) with
+  match NMap.find src st.(sent), NMap.find src st.(received) with
   | Some m_snt, Some m_rcd =>    
     put {| local := st.(local) ;
            aggregate := st.(aggregate) * m_snt * (m_rcd)^-1 ;
-           adjacent := FinNSet.remove src st.(adjacent) ;
-           sent := FinNMap.remove src st.(sent) ;
-           received := FinNMap.remove src st.(received) ;
+           adjacent := NSet.remove src st.(adjacent) ;
+           sent := NMap.remove src st.(sent) ;
+           received := NMap.remove src st.(received) ;
            broadcast := st.(broadcast) ;
            levels := st.(levels) |}
   | _, _ =>
     put {| local := st.(local) ;
            aggregate := st.(aggregate) ;
-           adjacent := FinNSet.remove src st.(adjacent) ;
+           adjacent := NSet.remove src st.(adjacent) ;
            sent := st.(sent) ;
            received := st.(received) ;
            broadcast := st.(broadcast) ;
@@ -378,26 +375,26 @@ Definition NonRootNetHandler (me src: name) (msg : Msg) : Handler Data :=
 st <- get ;;
 match msg with
 | Aggregate m_msg => 
-  match FinNMap.find src st.(received) with
+  match NMap.find src st.(received) with
   | None => nop
   | Some m_src => 
     put {| local := st.(local) ;
            aggregate := st.(aggregate) * m_msg ;
            adjacent := st.(adjacent) ;
            sent := st.(sent) ;
-           received := FinNMap.add src (m_src * m_msg) st.(received) ;
+           received := NMap.add src (m_src * m_msg) st.(received) ;
            broadcast := st.(broadcast) ;
            levels := st.(levels) |}
   end
 | Level None =>
-  if olv_eq_dec (level st.(adjacent) st.(levels)) (level st.(adjacent) (FinNMap.remove src st.(levels))) then
+  if olv_eq_dec (level st.(adjacent) st.(levels)) (level st.(adjacent) (NMap.remove src st.(levels))) then
     put {| local := st.(local) ;
            aggregate := st.(aggregate) ;
            adjacent := st.(adjacent) ;
            sent := st.(sent) ;
            received := st.(received) ;
            broadcast := st.(broadcast) ;
-           levels := FinNMap.remove src st.(levels) |}
+           levels := NMap.remove src st.(levels) |}
   else 
     put {| local := st.(local) ;
            aggregate := st.(aggregate) ;
@@ -405,16 +402,16 @@ match msg with
            sent := st.(sent) ;
            received := st.(received) ;
            broadcast := true ;
-           levels := FinNMap.remove src st.(levels) |}
+           levels := NMap.remove src st.(levels) |}
 | Level (Some lv') =>
-  if olv_eq_dec (level st.(adjacent) st.(levels)) (level st.(adjacent) (FinNMap.add src lv' st.(levels))) then
+  if olv_eq_dec (level st.(adjacent) st.(levels)) (level st.(adjacent) (NMap.add src lv' st.(levels))) then
     put {| local := st.(local) ;
            aggregate := st.(aggregate) ;
            adjacent := st.(adjacent) ;
            sent := st.(sent) ;
            received := st.(received) ;
            broadcast := st.(broadcast) ;
-           levels := FinNMap.add src lv' st.(levels) |}
+           levels := NMap.add src lv' st.(levels) |}
   else
     put {| local := st.(local) ;
            aggregate := st.(aggregate) ;
@@ -422,30 +419,30 @@ match msg with
            sent := st.(sent) ;
            received := st.(received) ;
            broadcast := true ;
-           levels := FinNMap.add src lv' st.(levels) |}
+           levels := NMap.add src lv' st.(levels) |}
 | Fail => 
-  match FinNMap.find src st.(sent), FinNMap.find src st.(received) with
+  match NMap.find src st.(sent), NMap.find src st.(received) with
   | Some m_snt, Some m_rcd =>    
-    if olv_eq_dec (level st.(adjacent) st.(levels)) (level (FinNSet.remove src st.(adjacent)) (FinNMap.remove src st.(levels))) then
+    if olv_eq_dec (level st.(adjacent) st.(levels)) (level (NSet.remove src st.(adjacent)) (NMap.remove src st.(levels))) then
       put {| local := st.(local) ;
              aggregate := st.(aggregate) * m_snt * (m_rcd)^-1 ;
-             adjacent := FinNSet.remove src st.(adjacent) ;
-             sent := FinNMap.remove src st.(sent) ;
-             received := FinNMap.remove src st.(received) ;
+             adjacent := NSet.remove src st.(adjacent) ;
+             sent := NMap.remove src st.(sent) ;
+             received := NMap.remove src st.(received) ;
              broadcast := st.(broadcast) ;
-             levels := FinNMap.remove src st.(levels) |}
+             levels := NMap.remove src st.(levels) |}
     else
       put {| local := st.(local) ;
              aggregate := st.(aggregate) * m_snt * (m_rcd)^-1 ;
-             adjacent := FinNSet.remove src st.(adjacent) ;
-             sent := FinNMap.remove src st.(sent) ;
-             received := FinNMap.remove src st.(received) ;
+             adjacent := NSet.remove src st.(adjacent) ;
+             sent := NMap.remove src st.(sent) ;
+             received := NMap.remove src st.(received) ;
              broadcast := true ;
-             levels := FinNMap.remove src st.(levels) |}
+             levels := NMap.remove src st.(levels) |}
   | _, _ => 
     put {| local := st.(local) ;
            aggregate := st.(aggregate) ;
-           adjacent := FinNSet.remove src st.(adjacent) ;
+           adjacent := NSet.remove src st.(adjacent) ;
            sent := st.(sent) ;
            received := st.(received) ;
            broadcast := st.(broadcast) ;
@@ -460,14 +457,14 @@ else NonRootNetHandler me src msg.
 Definition level_fold (lvo : option lv) (n : name) (partial : list (name * Msg)) : list (name * Msg) :=
 (n, Level lvo) :: partial.
 
-Definition level_adjacent (lvo : option lv) (fs : FinNS) : list (name * Msg) :=
-FinNSet.fold (level_fold lvo) fs [].
+Definition level_adjacent (lvo : option lv) (fs : NS) : list (name * Msg) :=
+NSet.fold (level_fold lvo) fs [].
 
 Definition send_level_fold (lvo : option lv) (n : name) (res : Handler Data) : Handler Data :=
 send (n, Level lvo) ;; res.
 
-Definition send_level_adjacent (lvo : option lv) (fs : FinNS) : Handler Data :=
-FinNSet.fold (send_level_fold lvo) fs nop.
+Definition send_level_adjacent (lvo : option lv) (fs : NS) : Handler Data :=
+NSet.fold (send_level_fold lvo) fs nop.
 
 Definition RootIOHandler (i : Input) : Handler Data :=
 st <- get ;;
@@ -513,14 +510,14 @@ match i with
   (match parent st.(adjacent) st.(levels) with
   | None => nop
   | Some dst => 
-    match FinNMap.find dst st.(sent) with
+    match NMap.find dst st.(sent) with
     | None => nop
     | Some m_dst =>   
       send (dst, (Aggregate st.(aggregate))) ;;
       put {| local := st.(local);
              aggregate := 1;
              adjacent := st.(adjacent);
-             sent := FinNMap.add dst (m_dst * st.(aggregate)) st.(sent);
+             sent := NMap.add dst (m_dst * st.(aggregate)) st.(sent);
              received := st.(received);
              broadcast := st.(broadcast);
              levels := st.(levels) |}
@@ -551,6 +548,23 @@ Instance TreeAggregation_BaseParams : BaseParams :=
     data := Data;
     input := Input;
     output := Output
+  }.
+
+Instance TreeAggregation_NameParams : NameParams :=
+  {
+    name := name ;
+    name_eq_dec := name_eq_dec ;
+    nodes := nodes ;
+    all_names_nodes := all_names_nodes ;
+    no_dup_nodes := no_dup_nodes
+  }.
+
+Instance TreeAggregation_NameOverlayParams : NameOverlayParams TreeAggregation_NameParams :=
+  {
+    adjacent_to := adjacent_to ;
+    adjacent_to_dec := adjacent_to_dec ;
+    adjacent_to_symmetric := adjacent_to_symmetric ;
+    adjacent_to_irreflexive := adjacent_to_irreflexive
   }.
 
 Instance TreeAggregation_MultiParams : MultiParams _ _ :=
@@ -586,55 +600,55 @@ Lemma NetHandler_cases :
   forall dst src msg st out st' ms,
     NetHandler dst src msg st = (tt, out, st', ms) ->
     (exists m_msg m_src, msg = Aggregate m_msg /\ 
-     FinNMap.find src st.(received) = Some m_src /\
+     NMap.find src st.(received) = Some m_src /\
      st'.(local) = st.(local) /\
      st'.(aggregate) = st.(aggregate) * m_msg /\
      st'.(adjacent) = st.(adjacent) /\
      st'.(sent) = st.(sent) /\     
-     st'.(received) = FinNMap.add src (m_src * m_msg) st.(received) /\
+     st'.(received) = NMap.add src (m_src * m_msg) st.(received) /\
      st'.(broadcast) = st.(broadcast) /\
      st'.(levels) = st.(levels) /\
      out = [] /\ ms = []) \/
     (exists m_msg, msg = Aggregate m_msg /\ 
-     FinNMap.find src st.(received) = None /\ 
+     NMap.find src st.(received) = None /\ 
      st' = st /\ 
      out = [] /\ ms = []) \/
     (root dst /\ msg = Fail /\ 
-     exists m_snt m_rcd, FinNMap.find src st.(sent) = Some m_snt /\ FinNMap.find src st.(received) = Some m_rcd /\
+     exists m_snt m_rcd, NMap.find src st.(sent) = Some m_snt /\ NMap.find src st.(received) = Some m_rcd /\
      st'.(local) = st.(local) /\ 
      st'.(aggregate) = st.(aggregate) * m_snt * (m_rcd)^-1 /\
-     st'.(adjacent) = FinNSet.remove src st.(adjacent) /\
-     st'.(sent) = FinNMap.remove src st.(sent) /\
-     st'.(received) = FinNMap.remove src st.(received) /\
+     st'.(adjacent) = NSet.remove src st.(adjacent) /\
+     st'.(sent) = NMap.remove src st.(sent) /\
+     st'.(received) = NMap.remove src st.(received) /\
      st'.(broadcast) = st.(broadcast) /\
      st'.(levels) = st.(levels) /\
      out = [] /\ ms = []) \/
     (~ root dst /\ msg = Fail /\ 
-     exists m_snt m_rcd, FinNMap.find src st.(sent) = Some m_snt /\ FinNMap.find src st.(received) = Some m_rcd /\
-     level st.(adjacent) st.(levels) = level (FinNSet.remove src st.(adjacent)) (FinNMap.remove src st.(levels)) /\
+     exists m_snt m_rcd, NMap.find src st.(sent) = Some m_snt /\ NMap.find src st.(received) = Some m_rcd /\
+     level st.(adjacent) st.(levels) = level (NSet.remove src st.(adjacent)) (NMap.remove src st.(levels)) /\
      st'.(local) = st.(local) /\ 
      st'.(aggregate) = st.(aggregate) * m_snt * (m_rcd)^-1 /\
-     st'.(adjacent) = FinNSet.remove src st.(adjacent) /\
-     st'.(sent) = FinNMap.remove src st.(sent) /\
-     st'.(received) = FinNMap.remove src st.(received) /\
+     st'.(adjacent) = NSet.remove src st.(adjacent) /\
+     st'.(sent) = NMap.remove src st.(sent) /\
+     st'.(received) = NMap.remove src st.(received) /\
      st'.(broadcast) = st.(broadcast) /\
-     st'.(levels) = FinNMap.remove src st.(levels) /\
+     st'.(levels) = NMap.remove src st.(levels) /\
      out = [] /\ ms = []) \/
     (~ root dst /\ msg = Fail /\ 
-     exists m_snt m_rcd, FinNMap.find src st.(sent) = Some m_snt /\ FinNMap.find src st.(received) = Some m_rcd /\
-     level st.(adjacent) st.(levels) <> level (FinNSet.remove src st.(adjacent)) (FinNMap.remove src st.(levels)) /\
+     exists m_snt m_rcd, NMap.find src st.(sent) = Some m_snt /\ NMap.find src st.(received) = Some m_rcd /\
+     level st.(adjacent) st.(levels) <> level (NSet.remove src st.(adjacent)) (NMap.remove src st.(levels)) /\
      st'.(local) = st.(local) /\ 
      st'.(aggregate) = st.(aggregate) * m_snt * (m_rcd)^-1 /\
-     st'.(adjacent) = FinNSet.remove src st.(adjacent) /\
-     st'.(sent) = FinNMap.remove src st.(sent) /\
-     st'.(received) = FinNMap.remove src st.(received) /\
+     st'.(adjacent) = NSet.remove src st.(adjacent) /\
+     st'.(sent) = NMap.remove src st.(sent) /\
+     st'.(received) = NMap.remove src st.(received) /\
      st'.(broadcast) = true /\
-     st'.(levels) = FinNMap.remove src st.(levels) /\
+     st'.(levels) = NMap.remove src st.(levels) /\
      out = [] /\ ms = []) \/
-    (msg = Fail /\ (FinNMap.find src st.(sent) = None \/ FinNMap.find src st.(received) = None) /\
+    (msg = Fail /\ (NMap.find src st.(sent) = None \/ NMap.find src st.(received) = None) /\
      st'.(local) = st.(local) /\ 
      st'.(aggregate) = st.(aggregate) /\
-     st'.(adjacent) = FinNSet.remove src st.(adjacent) /\
+     st'.(adjacent) = NSet.remove src st.(adjacent) /\
      st'.(sent) = st.(sent) /\
      st'.(received) = st.(received) /\
      st'.(broadcast) = st.(broadcast) /\
@@ -644,55 +658,55 @@ Lemma NetHandler_cases :
      st' = st /\
      out = [] /\ ms = []) \/
     (~ root dst /\ exists lv_msg, msg = Level (Some lv_msg) /\
-     level st.(adjacent) st.(levels) = level st.(adjacent) (FinNMap.add src lv_msg st.(levels)) /\
+     level st.(adjacent) st.(levels) = level st.(adjacent) (NMap.add src lv_msg st.(levels)) /\
      st'.(local) = st.(local) /\ 
      st'.(aggregate) = st.(aggregate) /\
      st'.(adjacent) = st.(adjacent) /\
      st'.(sent) = st.(sent) /\
      st'.(received) = st.(received) /\
      st'.(broadcast) = st.(broadcast) /\
-     st'.(levels) = FinNMap.add src lv_msg st.(levels) /\
+     st'.(levels) = NMap.add src lv_msg st.(levels) /\
      out = [] /\ ms = []) \/
     (~ root dst /\ exists lv_msg, msg = Level (Some lv_msg) /\
-     level st.(adjacent) st.(levels) <> level st.(adjacent) (FinNMap.add src lv_msg st.(levels)) /\
+     level st.(adjacent) st.(levels) <> level st.(adjacent) (NMap.add src lv_msg st.(levels)) /\
      st'.(local) = st.(local) /\ 
      st'.(aggregate) = st.(aggregate) /\
      st'.(adjacent) = st.(adjacent) /\
      st'.(sent) = st.(sent) /\
      st'.(received) = st.(received) /\
      st'.(broadcast) = true /\
-     st'.(levels) = FinNMap.add src lv_msg st.(levels) /\
+     st'.(levels) = NMap.add src lv_msg st.(levels) /\
      out = [] /\ ms = []) \/
     (~ root dst /\ msg = Level None /\
-     level st.(adjacent) st.(levels) = level st.(adjacent) (FinNMap.remove src st.(levels)) /\
+     level st.(adjacent) st.(levels) = level st.(adjacent) (NMap.remove src st.(levels)) /\
      st'.(local) = st.(local) /\ 
      st'.(aggregate) = st.(aggregate) /\
      st'.(adjacent) = st.(adjacent) /\
      st'.(sent) = st.(sent) /\
      st'.(received) = st.(received) /\
      st'.(broadcast) = st.(broadcast) /\
-     st'.(levels) = FinNMap.remove src st.(levels) /\
+     st'.(levels) = NMap.remove src st.(levels) /\
      out = [] /\ ms = []) \/
     (~ root dst /\ msg = Level None /\
-     level st.(adjacent) st.(levels) <> level st.(adjacent) (FinNMap.remove src st.(levels)) /\
+     level st.(adjacent) st.(levels) <> level st.(adjacent) (NMap.remove src st.(levels)) /\
      st'.(local) = st.(local) /\ 
      st'.(aggregate) = st.(aggregate) /\
      st'.(adjacent) = st.(adjacent) /\
      st'.(sent) = st.(sent) /\
      st'.(received) = st.(received) /\
      st'.(broadcast) = true /\
-     st'.(levels) = FinNMap.remove src st.(levels) /\
+     st'.(levels) = NMap.remove src st.(levels) /\
      out = [] /\ ms = []).
 Proof.
 move => dst src msg st out st' ms.
 rewrite /NetHandler /RootNetHandler /NonRootNetHandler.
 case: msg => [m_msg||olv_msg]; monad_unfold.
-- case root_dec => /= H_dec; case H_find: (FinNMap.find _ _) => [m_src|] /= H_eq; injection H_eq => H_ms H_st H_out; rewrite -H_st /=.
+- case root_dec => /= H_dec; case H_find: (NMap.find _ _) => [m_src|] /= H_eq; injection H_eq => H_ms H_st H_out; rewrite -H_st /=.
   * by left; exists m_msg; exists m_src.
   * by right; left; exists m_msg.
   * by left; exists m_msg; exists m_src.
   * by right; left; exists m_msg.
-- case root_dec => /= H_dec; case H_find: (FinNMap.find _ _) => [m_snt|]; case H_find': (FinNMap.find _ _) => [m_rcd|] /=.
+- case root_dec => /= H_dec; case H_find: (NMap.find _ _) => [m_snt|]; case H_find': (NMap.find _ _) => [m_rcd|] /=.
   * move => H_eq.
     injection H_eq => H_ms H_st H_out; rewrite -H_st /=.
     right; right; left.
@@ -786,10 +800,10 @@ Qed.
 Lemma send_level_fold_app :
   forall ns st olv nm,
 snd (fold_left 
-       (fun (a : Handler Data) (e : FinNSet.elt) => send_level_fold olv e a) ns
+       (fun (a : Handler Data) (e : NSet.elt) => send_level_fold olv e a) ns
        (fun s : Data => (tt, [], s, nm)) st) = 
 snd (fold_left 
-       (fun (a : Handler Data) (e : FinNSet.elt) => send_level_fold olv e a) ns
+       (fun (a : Handler Data) (e : NSet.elt) => send_level_fold olv e a) ns
        (fun s : Data => (tt, [], s, [])) st) ++ nm.
 Proof.
 elim => //=.
@@ -808,9 +822,9 @@ forall fs olv st,
 Proof.
 move => fs olv st.
 rewrite /send_level_adjacent /level_adjacent.
-rewrite 2!FinNSet.fold_spec.
+rewrite 2!NSet.fold_spec.
 move: olv st.
-elim: FinNSet.elements => [|n ns IH] //=.
+elim: NSet.elements => [|n ns IH] //=.
 move => olv st.
 rewrite {2}/level_fold {2}/send_level_fold.
 rewrite fold_left_level_fold_eq.
@@ -826,7 +840,7 @@ fst
   (fst
      (fst
         (fold_left
-           (fun (a : Handler Data) (e : FinNSet.elt) =>
+           (fun (a : Handler Data) (e : NSet.elt) =>
               send_level_fold olv e a) ns
            (fun s : Data => (tt, [], s, nm)) st))) = tt.
 Proof.
@@ -841,7 +855,7 @@ forall fs olv st,
 Proof.
 move => fs olv st.
 rewrite /send_level_adjacent.
-rewrite FinNSet.fold_spec.
+rewrite NSet.fold_spec.
 by rewrite fst_fst_fst_tt_send_level_fold.
 Qed.
 
@@ -851,7 +865,7 @@ snd
   (fst
      (fst
         (fold_left
-           (fun (a : Handler Data) (e : FinNSet.elt) =>
+           (fun (a : Handler Data) (e : NSet.elt) =>
               send_level_fold olv e a) ns
            (fun s : Data => (tt, [], s, nm)) st))) = [].
 Proof.
@@ -864,7 +878,7 @@ Lemma snd_fst_st_send_level_fold :
 forall ns nm olv st,
 snd (fst
         (fold_left
-           (fun (a : Handler Data) (e : FinNSet.elt) =>
+           (fun (a : Handler Data) (e : NSet.elt) =>
               send_level_fold olv e a) ns
            (fun s : Data => (tt, [], s, nm)) st)) = st.
 Proof.
@@ -879,7 +893,7 @@ forall fs olv st,
 Proof.
 move => fs olv st.
 rewrite /send_level_adjacent.
-rewrite FinNSet.fold_spec.
+rewrite NSet.fold_spec.
 by rewrite snd_fst_fst_out_send_level_fold.
 Qed.
 
@@ -889,7 +903,7 @@ forall fs olv st,
 Proof.
 move => fs olv st.
 rewrite /send_level_adjacent.
-rewrite FinNSet.fold_spec.
+rewrite NSet.fold_spec.
 by rewrite snd_fst_st_send_level_fold.
 Qed.
 
@@ -927,11 +941,11 @@ Lemma IOHandler_cases :
          out = [] /\ ms = []) \/
       (~ root h /\ i = SendAggregate /\ 
        st.(aggregate) <> 1 /\ 
-       exists dst m_dst, parent st.(adjacent) st.(levels) = Some dst /\ FinNMap.find dst st.(sent) = Some m_dst /\
+       exists dst m_dst, parent st.(adjacent) st.(levels) = Some dst /\ NMap.find dst st.(sent) = Some m_dst /\
        st'.(local) = st.(local) /\
        st'.(aggregate) = 1 /\ 
        st'.(adjacent) = st.(adjacent) /\
-       st'.(sent) = FinNMap.add dst (m_dst * st.(aggregate)) st.(sent) /\
+       st'.(sent) = NMap.add dst (m_dst * st.(aggregate)) st.(sent) /\
        st'.(received) = st.(received) /\
        st'.(broadcast) = st.(broadcast) /\
        st'.(levels) = st.(levels) /\
@@ -947,7 +961,7 @@ Lemma IOHandler_cases :
        out = [] /\ ms = []) \/
       (~ root h /\ i = SendAggregate /\
        st.(aggregate) <> 1 /\
-       exists dst, parent st.(adjacent) st.(levels) = Some dst /\ FinNMap.find dst st.(sent) = None /\ 
+       exists dst, parent st.(adjacent) st.(levels) = Some dst /\ NMap.find dst st.(sent) = None /\ 
        st' = st /\
        out = [] /\ ms = []) \/
       (i = AggregateRequest /\ 
@@ -991,7 +1005,7 @@ case: i => [m_msg||||]; monad_unfold.
     by move => H_eq; injection H_eq => H_ms H_st H_out H_tt; rewrite -H_st /=; right; right; right; left.
   case H_p: parent => [dst|]; last first. 
     by move => H_eq; injection H_eq => H_ms H_st H_out H_tt; rewrite -H_st /=; right; right; right; right; left.
-  case H_find: FinNMap.find => [m_dst|] H_eq; injection H_eq => H_ms H_st H_out H_tt; rewrite -H_st /=.
+  case H_find: NMap.find => [m_dst|] H_eq; injection H_eq => H_ms H_st H_out H_tt; rewrite -H_st /=.
     right; right; left.
     split => //.
     split => //.
@@ -1055,7 +1069,7 @@ Ltac io_handler_cases :=
   intuition idtac; subst; 
   repeat find_rewrite.
 
-Instance TreeAggregation_Aggregation_name_params_tot_map : NameParamsTotalMap Fin_n_NameParams AGN.FRN.AN.Fin_n_NameParams :=
+Instance TreeAggregation_Aggregation_name_params_tot_map : NameParamsTotalMap TreeAggregation_NameParams AGN.Aggregation_NameParams :=
   {
     tot_map_name := id ;
     tot_map_name_inv := id
@@ -1097,7 +1111,7 @@ Lemma tot_map_name_inverse_inv : forall n, tot_map_name (tot_map_name_inv n) = n
 Proof. by []. Qed.
 
 Lemma pt_ext_init_handlers_eq : forall n,
-  @pt_ext_map_data _ _ _ _ _ _ _ TreeAggregation_Aggregation_params_pt_ext_map (init_handlers n) n = @init_handlers _ _ AGN.Aggregation_MultiParams (tot_map_name n).
+  pt_ext_map_data (init_handlers n) n = init_handlers (tot_map_name n).
 Proof.
 move => n.
 rewrite /= /InitData /=.
@@ -1105,8 +1119,8 @@ by case root_dec => /= H_dec.
 Qed.
 
 Lemma pt_ext_net_handlers_some : forall me src m st m',
-  @pt_ext_map_msg _ _ _ _ _ _ _ TreeAggregation_Aggregation_params_pt_ext_map m = Some m' ->
-  pt_ext_mapped_net_handlers me src m st = net_handlers (tot_map_name me) (tot_map_name src) m' (@pt_ext_map_data _ _ _ _ _ _ _ TreeAggregation_Aggregation_params_pt_ext_map st me).
+  pt_ext_map_msg m = Some m' ->
+  pt_ext_mapped_net_handlers me src m st = net_handlers (tot_map_name me) (tot_map_name src) m' (pt_ext_map_data st me).
 Proof.
 move => me src.
 case => //.
@@ -1129,7 +1143,7 @@ case => //.
     monad_unfold.
     break_let.
     move: Heqp2.
-    case H_find: FinNMap.find => /= [m0|]; last by rewrite H in H_find.
+    case H_find: NMap.find => /= [m0|]; last by rewrite H in H_find.
     rewrite H in H_find.
     injection H_find => H_eq_m.
     rewrite H_eq_m.
@@ -1145,7 +1159,7 @@ case => //.
   monad_unfold.
   break_let.
   move: Heqp2.
-  case H_find: FinNMap.find => /= [m0|]; first by rewrite H in H_find.
+  case H_find: NMap.find => /= [m0|]; first by rewrite H in H_find.
   repeat break_let.
   move => Heqp Heqp'.
   rewrite Heqp' in Heqp.
@@ -1168,8 +1182,8 @@ net_handler_cases => //.
   monad_unfold.
   break_let.
   move: Heqp2.
-  case H_find: FinNMap.find => /= [m0|]; last by rewrite H2 in H_find.
-  case H_find': FinNMap.find => /= [m1|]; last by rewrite H1 in H_find'.
+  case H_find: NMap.find => /= [m0|]; last by rewrite H2 in H_find.
+  case H_find': NMap.find => /= [m1|]; last by rewrite H1 in H_find'.
   rewrite H2 in H_find.
   injection H_find => H_eq_m.
   rewrite H_eq_m.
@@ -1188,8 +1202,8 @@ net_handler_cases => //.
   monad_unfold.
   break_let.
   move: Heqp2.
-  case H_find: FinNMap.find => /= [m0|]; last by rewrite H2 in H_find.
-  case H_find': FinNMap.find => /= [m1|]; last by rewrite H1 in H_find'.
+  case H_find: NMap.find => /= [m0|]; last by rewrite H2 in H_find.
+  case H_find': NMap.find => /= [m1|]; last by rewrite H1 in H_find'.
   rewrite H2 in H_find.
   injection H_find => H_eq_m.
   rewrite H_eq_m.
@@ -1208,8 +1222,8 @@ net_handler_cases => //.
   monad_unfold.
   break_let.
   move: Heqp2.
-  case H_find: FinNMap.find => /= [m0|]; last by rewrite H2 in H_find.
-  case H_find': FinNMap.find => /= [m1|]; last by rewrite H1 in H_find'.
+  case H_find: NMap.find => /= [m0|]; last by rewrite H2 in H_find.
+  case H_find': NMap.find => /= [m1|]; last by rewrite H1 in H_find'.
   rewrite H2 in H_find.
   injection H_find => H_eq_m.
   rewrite H_eq_m.
@@ -1228,7 +1242,7 @@ net_handler_cases => //.
   monad_unfold.
   break_let.
   move: Heqp2.
-  case H_find: FinNMap.find => /= [m0|]; first by rewrite H9 in H_find.
+  case H_find: NMap.find => /= [m0|]; first by rewrite H9 in H_find.
   repeat break_let.
   move => Heqp Heqp'.      
   rewrite Heqp' in Heqp.
@@ -1242,8 +1256,8 @@ net_handler_cases => //.
   break_let.
   move: Heqp2.
   rewrite /=.
-  case H_find': (FinNMap.find _  st.(received)) => /= [m1|]; first by rewrite H9 in H_find'.
-  case H_find: FinNMap.find => /= [m0|].
+  case H_find': (NMap.find _  st.(received)) => /= [m1|]; first by rewrite H9 in H_find'.
+  case H_find: NMap.find => /= [m0|].
     repeat break_let.
     move => Heqp Heqp'.      
     rewrite Heqp' in Heqp.
@@ -1255,9 +1269,9 @@ net_handler_cases => //.
 Qed.
 
 Lemma pt_ext_net_handlers_none : forall me src m st out st' ps,
-  @pt_ext_map_msg _ _ _ _ _ _ _ TreeAggregation_Aggregation_params_pt_ext_map m = None ->
+  pt_ext_map_msg m = None ->
   net_handlers me src m st = (out, st', ps) ->
-  @pt_ext_map_data _ _ _ _ _ _ _ TreeAggregation_Aggregation_params_pt_ext_map st' me = @pt_ext_map_data _ _ _ _ _ _ _ TreeAggregation_Aggregation_params_pt_ext_map st me /\ @pt_ext_map_name_msgs _ _ _ _ _ _ _ TreeAggregation_Aggregation_params_pt_ext_map ps = [].
+  pt_ext_map_data st' me = pt_ext_map_data st me /\ pt_ext_map_name_msgs ps = [].
 Proof.
 move => me src.
 case => //.
@@ -1282,8 +1296,6 @@ net_handler_cases => //.
   by rewrite H2 H3 H4 H5 H6.
 Qed.
 
-(* BLA *)
-
 Lemma pt_ext_input_handlers_some : forall me inp st inp',
   pt_ext_map_input inp me st = Some inp' ->
   pt_ext_mapped_input_handlers me inp st = input_handlers (tot_map_name me) inp' (pt_ext_map_data st me).
@@ -1305,7 +1317,7 @@ case => //.
   move: Heqp.
   injection H0 => H_eq_m.
   rewrite -H_eq_m {H_eq_m H0}.
-  rewrite /AM.IOHandler.
+  rewrite /AGN.IOHandler.
   monad_unfold.
   rewrite /=.
   move => Heqp.
@@ -1341,16 +1353,16 @@ case => //.
       monad_unfold.
       repeat break_let.
       move: Heqp.      
-      rewrite /AM.IOHandler.
+      rewrite /AGN.IOHandler.
       monad_unfold.
       rewrite /=.
       repeat break_let.
       move: Heqp2.
-      case H_mem: FinNSet.mem => /=; last by move/negP: H_mem => H_mem; case: H_mem; apply FinNSetFacts.mem_1.
+      case H_mem: NSet.mem => /=; last by move/negP: H_mem => H_mem; case: H_mem; apply NSetFacts.mem_1.
       case sumbool_not => //= H_not.
       repeat break_let.
       move: Heqp2.
-      case H_find: AM.FinNMap.find => [m0|]; last by rewrite H_find in H6.
+      case H_find: NMap.find => [m0|]; last by rewrite H_find in H6.
       rewrite H_find in H6.
       injection H6 => H_eq'.
       rewrite H_eq'.
@@ -1363,11 +1375,11 @@ case => //.
     * monad_unfold.
       repeat break_let.
       move: Heqp.      
-      rewrite /AM.IOHandler.
+      rewrite /AGN.IOHandler.
       monad_unfold.
       repeat break_let.
       move: Heqp2.
-      case H_mem: FinNSet.mem => /=; last by move/negP: H_mem => H_mem; case: H_mem; apply FinNSetFacts.mem_1.
+      case H_mem: NSet.mem => /=; last by move/negP: H_mem => H_mem; case: H_mem; apply NSetFacts.mem_1.
       case sumbool_not => //= H_not.
       move => H_eq H_eq'.
       rewrite H_eq' in H_eq.
@@ -1377,15 +1389,15 @@ case => //.
       monad_unfold.
       repeat break_let.
       move: Heqp.
-      rewrite /AM.IOHandler.
+      rewrite /AGN.IOHandler.
       monad_unfold.
       repeat break_let.
       move: Heqp2.
-      case H_mem: FinNSet.mem => /=; last by move/negP: H_mem => H_mem; case: H_mem; apply FinNSetFacts.mem_1.
+      case H_mem: NSet.mem => /=; last by move/negP: H_mem => H_mem; case: H_mem; apply NSetFacts.mem_1.
       case sumbool_not => //= H_not.
       repeat break_let.
       move: Heqp2.
-      case H_find: AM.FinNMap.find => [m0|]; first by rewrite H_find in H6.
+      case H_find: NMap.find => [m0|]; first by rewrite H_find in H6.
       rewrite -2!app_nil_end.
       move => H_eq_1 H_eq_2 H_eq3.
       inversion H_eq3; subst.
@@ -1407,8 +1419,8 @@ Lemma pt_ext_map_name_msgs_level_adjacent_empty :
   pt_ext_map_name_msgs (level_adjacent lvo fs) = [].
 Proof.
 move => fs lvo.
-rewrite /level_adjacent FinNSet.fold_spec.
-elim: FinNSet.elements => //=.
+rewrite /level_adjacent NSet.fold_spec.
+elim: NSet.elements => //=.
 move => n ns IH.
 rewrite {2}/level_fold /=.
 rewrite fold_left_level_fold_eq /=.
@@ -1455,16 +1467,16 @@ Lemma fail_msg_fst_snd : pt_ext_map_msg msg_fail = Some (msg_fail).
 Proof. by []. Qed.
 
 Lemma adjacent_to_fst_snd : 
-  forall n n', adjacent_to n n' <-> adjacent_to (pt_ext_map_name n) (pt_ext_map_name n').
+  forall n n', adjacent_to n n' <-> adjacent_to (tot_map_name n) (tot_map_name n').
 Proof. by []. Qed.
 
 Theorem TreeAggregation_Aggregation_pt_ext_mapped_simulation_star_1 :
 forall net failed tr,
-    @step_o_f_star _ _ TreeAggregation_OverlayParams TreeAggregation_FailMsgParams step_o_f_init (failed, net) tr ->
-    exists tr', @step_o_f_star _ _ AM.Aggregation_OverlayParams AM.Aggregation_FailMsgParams step_o_f_init (failed, pt_ext_map_onet net) tr'.
+    @step_o_f_star _ _ _ TreeAggregation_NameOverlayParams TreeAggregation_FailMsgParams step_o_f_init (failed, net) tr ->
+    exists tr', @step_o_f_star _ _ _ AGN.Aggregation_NameOverlayParams AGN.Aggregation_FailMsgParams step_o_f_init (failed, pt_ext_map_onet net) tr'.
 Proof.
-have H_sim := step_o_f_pt_ext_mapped_simulation_star_1 pt_ext_map_name_inv_inverse pt_ext_map_name_inverse_inv pt_ext_init_handlers_eq pt_ext_net_handlers_some pt_ext_net_handlers_none pt_ext_input_handlers_some pt_ext_input_handlers_none adjacent_to_fst_snd fail_msg_fst_snd.
-rewrite /pt_ext_map_name /= /id in H_sim.
+have H_sim := @step_o_f_pt_ext_mapped_simulation_star_1 _ _ _  _ _ _ _ _ tot_map_name_inverse_inv tot_map_name_inv_inverse pt_ext_init_handlers_eq pt_ext_net_handlers_some pt_ext_net_handlers_none pt_ext_input_handlers_some pt_ext_input_handlers_none TreeAggregation_NameOverlayParams TreeAggregation_NameOverlayParams adjacent_to_fst_snd _ _ fail_msg_fst_snd.
+rewrite /tot_map_name /= /id in H_sim.
 move => onet failed tr H_st.
 apply H_sim in H_st.
 move: H_st => [tr' H_st].
